Locks: Adjust interface, add library code.
Interface: support progress bits, make newlock' the primitive.

Libraries: newlock, sync_with, make_sync.

theories/heap_lang/lib/lock.v
@@ -1,9 +1,12 @@
 From iris.heap_lang Require Export heap notation.
-From iris.base_logic.lib Require Export invariants.
+From iris.heap_lang Require Import proofmode.
+From iris.proofmode Require Import tactics.
+Import uPred.
 
+(** * Lock interface *)
 Structure lock Σ `{!heapG Σ} := Lock {
   (* -- operations -- *)
-  newlock : val;
+  newlock' : val;
   acquire : val;
   release : val;
   (* -- predicates -- *)
@@ -17,16 +20,17 @@ Structure lock Σ `{!heapG Σ} := Lock {
   locked_timeless γ : TimelessP (locked γ);
   locked_exclusive γ : locked γ -∗ locked γ -∗ False;
   (* -- operation specs -- *)
-  newlock_spec N (R : iProp Σ) :
+  newlock'_spec p N (R : iProp Σ) :
     heapN ⊥ N →
-    {{{ heap_ctx ∗ R }}} newlock #() {{{ lk γ, RET lk; is_lock N γ lk R }}};
-  acquire_spec N γ lk R :
-    {{{ is_lock N γ lk R }}} acquire lk {{{ RET #(); locked γ ∗ R }}};
-  release_spec N γ lk R :
-    {{{ is_lock N γ lk R ∗ locked γ ∗ R }}} release lk {{{ RET #(); True }}}
+    {{{ heap_ctx }}} newlock' #() @ p; ⊤
+    {{{ lk γ, RET lk;  is_lock N γ lk R ∗ locked γ }}};
+  acquire_spec p N γ lk R :
+    {{{ is_lock N γ lk R }}} acquire lk @ p; ⊤ {{{ RET #(); locked γ ∗ R }}};
+  release_spec p N γ lk R :
+    {{{ is_lock N γ lk R ∗ locked γ ∗ R }}} release lk @ p; ⊤ {{{ RET #(); True }}}
 }.
 
-Arguments newlock {_ _} _.
+Arguments newlock' {_ _} _.
 Arguments acquire {_ _} _.
 Arguments release {_ _} _.
 Arguments is_lock {_ _} _ _ _ _ _.
@@ -37,3 +41,76 @@ Existing Instances is_lock_ne is_lock_persistent locked_timeless.
 Instance is_lock_proper Σ `{!heapG Σ} (L: lock Σ) N lk R:
   Proper ((≡) ==> (≡)) (is_lock L N lk R) := ne_proper _.
 
+(** * The [newlock] function *)
+Section newlock.
+  Context `{heapG Σ} (L : lock Σ).
+
+  Definition newlock : val := λ: <>,
+    let: "lk" := newlock' L #() in release L "lk" ;; "lk".
+
+  Lemma newlock_spec p N (R : iProp Σ) :
+    heapN ⊥ N →
+    {{{ heap_ctx ∗ R }}} newlock #() @ p; ⊤
+    {{{ lk γ, RET lk; is_lock L N γ lk R }}}.
+  Proof.
+    iIntros (? Φ) "[#Hh Hr] HΦ"; wp_lam.
+    wp_bind (newlock' _ _); iApply (newlock'_spec _ _ _ _ R with "[$Hh]");
+      first done; iNext; iIntros (lk γ) "[#Hlk Hl]"; wp_let.
+    wp_bind (release _ _); iApply (release_spec with "[$Hlk $Hl $Hr]"); iNext;
+      iIntros "_"; wp_seq.
+    by iApply ("HΦ" with "[$Hlk]").
+  Qed.
+End newlock.
+
+(** * The [sync_with] and [make_sync] functions *)
+Section sync.
+  Context `{heapG Σ} (L : lock Σ).
+
+  Definition sync_with : val := λ: "lk" "f",
+    acquire L "lk" ;; let: "r" := "f" #() in release L "lk" ;; "r".
+  Definition make_sync : val := λ: <>,
+    let: "lk" := newlock L #() in sync_with "lk".
+
+  Definition is_sync (sync : val) (R : iProp Σ) : iProp Σ := (
+    □ ∀ p e Φ, ⌜Closed [] e⌝ -∗
+    (∀ Ψ, R -∗ ▷ (∀ v, R -∗ Φ v -∗ Ψ v) -∗ WP e @ p; ⊤{{ Ψ }}) -∗
+    WP sync (λ: <>, e) @ p; ⊤{{ Φ }}
+  )%I.
+
+  Global Instance is_sync_persistent v R : PersistentP (is_sync v R).
+  Proof. apply _. Qed.
+
+  Global Instance is_sync_ne n v : Proper (dist n ==> dist n) (is_sync v).
+  Proof. solve_proper. Qed.
+
+  Lemma sync_with_spec p N γ lk (R : iProp Σ) :
+    {{{ is_lock L N γ lk R }}} sync_with lk @ p; ⊤
+    {{{ sync, RET sync; is_sync sync R }}}.
+  Proof.
+    iIntros (Φ) "#Hlk HΦ". wp_lam.
+    iApply "HΦ". iAlways. iIntros (p' e ψ) "% He". wp_let.
+    wp_bind (acquire _ _). iApply (acquire_spec with "Hlk"). iNext.
+      iIntros "[Hlocked Hr]". wp_seq. wp_let.
+    iApply ("He" with "[$Hr]"). iNext. iIntros (v) "Hr HΨ". wp_let.
+    wp_bind (release _ _). iApply (release_spec with "[$Hlk $Hlocked $Hr]").
+      iNext. rewrite wand_True. wp_seq. iExact "HΨ".
+  Qed.
+
+  Lemma make_sync_spec p N (R : iProp Σ) :
+    heapN ⊥ N →
+    {{{ heap_ctx ∗ R }}} make_sync #() @ p; ⊤
+    {{{ sync, RET sync; is_sync sync R }}}.
+  Proof.
+    iIntros (? Φ) "[#Hh HR] HΦ"; wp_lam.
+    wp_bind (newlock _ _);
+      iApply (newlock_spec _ _ _ R with "[$Hh $HR]"); first done;
+      iNext; iIntros (lk γ) "#Hlk"; wp_let.
+    by iApply (sync_with_spec with "[$Hlk] [$HΦ]").
+  Qed.
+End sync.
+
+Typeclasses Opaque is_sync.
+Instance: Params (@is_sync) 2.
+
+Instance is_sync_proper Σ `{heapG Σ} sync :
+  Proper ((≡) ==> (≡)) (is_sync sync) := ne_proper _.
