theories/heap_lang/lib/spin_lock.v
@@ -5,7 +5,7 @@ From iris.heap_lang Require Import proofmode notation.
 From iris.algebra Require Import excl.
 From iris.heap_lang.lib Require Import lock.
 
-Definition newlock : val := λ: <>, ref #false.
+Definition newlock' : val := λ: <>, ref #true.
 Definition try_acquire : val := λ: "l", CAS "l" #false #true.
 Definition acquire : val :=
   rec: "acquire" "l" := if: try_acquire "l" then #() else "acquire" "l".
@@ -20,7 +20,7 @@ Instance subG_lockΣ {Σ} : subG lockΣ Σ → lockG Σ.
 Proof. intros [?%subG_inG _]%subG_inv. split; apply _. Qed.
 
 Section proof.
-  Context `{!heapG Σ, !lockG Σ} (N : namespace).
+  Context `{!heapG Σ, !lockG Σ} (p : pbit) (N : namespace).
 
   Definition lock_inv (γ : gname) (l : loc) (R : iProp Σ) : iProp Σ :=
     (∃ b : bool, l ↦ #b ∗ if b then True else own γ (Excl ()) ∗ R)%I.
@@ -44,20 +44,21 @@ Section proof.
   Global Instance locked_timeless γ : TimelessP (locked γ).
   Proof. apply _. Qed.
 
-  Lemma newlock_spec (R : iProp Σ):
+  Lemma newlock'_spec (R : iProp Σ):
     heapN ⊥ N →
-    {{{ heap_ctx ∗ R }}} newlock #() {{{ lk γ, RET lk; is_lock γ lk R }}}.
+    {{{ heap_ctx }}} newlock' #() @ p; ⊤
+    {{{ lk γ, RET lk; is_lock γ lk R ∗ locked γ }}}.
   Proof.
-    iIntros (? Φ) "[#Hh HR] HΦ". rewrite -wp_fupd /newlock /=.
+    iIntros (? Φ) "#Hh HΦ". rewrite -wp_fupd /newlock /=.
     wp_seq. wp_alloc l as "Hl".
     iMod (own_alloc (Excl ())) as (γ) "Hγ"; first done.
-    iMod (inv_alloc N _ (lock_inv γ l R) with "[-HΦ]") as "#?".
-    { iIntros "!>". iExists false. by iFrame. }
-    iModIntro. iApply "HΦ". iExists l. eauto.
+    iMod (inv_alloc N _ (lock_inv γ l R) with "[Hl]") as "#?".
+    { iIntros "!>". iExists true. by iFrame. }
+    iModIntro. iApply "HΦ". iSplitR "Hγ". by iExists l; eauto. by iFrame.
   Qed.
 
   Lemma try_acquire_spec γ lk R :
-    {{{ is_lock γ lk R }}} try_acquire lk
+    {{{ is_lock γ lk R }}} try_acquire lk @ p; ⊤
     {{{ b, RET #b; if b is true then locked γ ∗ R else True }}}.
   Proof.
     iIntros (Φ) "#Hl HΦ". iDestruct "Hl" as (l) "(% & #? & % & #?)"; subst.
@@ -70,7 +71,7 @@ Section proof.
   Qed.
 
   Lemma acquire_spec γ lk R :
-    {{{ is_lock γ lk R }}} acquire lk {{{ RET #(); locked γ ∗ R }}}.
+    {{{ is_lock γ lk R }}} acquire lk @ p; ⊤ {{{ RET #(); locked γ ∗ R }}}.
   Proof.
     iIntros (Φ) "#Hl HΦ". iLöb as "IH". wp_rec.
     wp_apply (try_acquire_spec with "Hl"). iIntros ([]).
@@ -79,7 +80,7 @@ Section proof.
   Qed.
 
   Lemma release_spec γ lk R :
-    {{{ is_lock γ lk R ∗ locked γ ∗ R }}} release lk {{{ RET #(); True }}}.
+    {{{ is_lock γ lk R ∗ locked γ ∗ R }}} release lk @ p; ⊤ {{{ RET #(); True }}}.
   Proof.
     iIntros (Φ) "(Hlock & Hlocked & HR) HΦ".
     iDestruct "Hlock" as (l) "(% & #? & % & #?)"; subst.
@@ -91,5 +92,5 @@ End proof.
 Typeclasses Opaque is_lock locked.
 
 Definition spin_lock `{!heapG Σ, !lockG Σ} : lock Σ :=
-  {| lock.locked_exclusive := locked_exclusive; lock.newlock_spec := newlock_spec;
+  {| lock.locked_exclusive := locked_exclusive; lock.newlock'_spec := newlock'_spec;
      lock.acquire_spec := acquire_spec; lock.release_spec := release_spec |}.
